well formedness preserved

dev/map/Map.v
@@ -1,12 +1,36 @@
 Require Import Fsub.
 Require Import Dsub.
 
+Set Implicit Arguments.
+Require Import LibLN.
+Implicit Types x : var.
+Implicit Types X : var.
+
+(* to adjust the bound identifier when shifting from a plain arrow to an all type *)
+Fixpoint inc_bound_rec (k: nat) (T : typ) {struct T} : typ :=
+  match T with
+  | typ_top         => typ_top
+  | typ_sel t       => typ_sel (inc_bound_e_rec k t)
+  | typ_mem b T     => typ_mem b (inc_bound_rec k T)
+  | typ_all T1 T2   => typ_all (inc_bound_rec k T1) (inc_bound_rec (S k) T2)
+  end
+with inc_bound_e_rec (k: nat) (e : trm) {struct e} : trm :=
+  match e with
+  | trm_bvar i    => trm_bvar (If (k <= i) then (S i) else i)
+  | trm_fvar x    => trm_fvar x
+  | trm_abs V e1  => trm_abs (inc_bound_rec k V) (inc_bound_e_rec (S k) e1)
+  | trm_mem T     => trm_mem (inc_bound_rec k T)
+  | trm_app e1 e2 => trm_app (inc_bound_e_rec k e1) (inc_bound_e_rec k e2)
+  end.
+
+Definition inc_bound T := inc_bound_rec 0 T.
+
 Fixpoint emb_t (T: Fsub.typ): Dsub.typ :=
   match T with
     | Fsub.typ_top => typ_top
     | Fsub.typ_bvar i => typ_sel (trm_bvar i)
     | Fsub.typ_fvar x => typ_sel (trm_fvar x)
-    | Fsub.typ_arrow T U => typ_all (emb_t T) (emb_t U)
+    | Fsub.typ_arrow T U => typ_all (emb_t T) (inc_bound (emb_t U))
     | Fsub.typ_all T U => typ_all (typ_mem false (emb_t T)) (emb_t U)
   end.
 
@@ -19,3 +43,131 @@ Fixpoint emb_e (e: Fsub.trm): Dsub.trm :=
     | Fsub.trm_app e1 e2 => trm_app (emb_e e1) (emb_e e2)
     | Fsub.trm_tapp e1 U => trm_app (emb_e e1) (trm_mem (emb_t U))
   end.
+
+Definition emb_tb (b: bind): Dsub.typ :=
+  match b with
+    | bind_sub T => typ_mem false (emb_t T)
+    | bind_typ T => emb_t T
+  end.
+
+Definition emb_env (E: Fsub.env): Dsub.env := map emb_tb E.
+
+Lemma binds_preserved: forall X b E,
+  binds X b E ->
+  binds X (emb_tb b) (emb_env E).
+Proof.
+  intros. apply* binds_map.
+Qed.
+
+Lemma binds_sub_preserved: forall X U E,
+  binds X (bind_sub U) E ->
+  binds X (typ_mem false (emb_t U)) (emb_env E).
+Proof.
+  intros. apply binds_preserved in H. simpl in H. apply H.
+Qed.
+
+Lemma binds_typ_preserved: forall X U E,
+  binds X (bind_typ U) E ->
+  binds X (emb_t U) (emb_env E).
+Proof.
+  intros. apply binds_preserved in H. simpl in H. apply H.
+Qed.
+
+Lemma inc_bound_open_commute_rec:
+  (forall T y n k, k <= n ->
+     inc_bound_rec k (open_t_rec n (trm_fvar y) T) =
+     open_t_rec (S n) (trm_fvar y) (inc_bound_rec k T))
+  /\
+  (forall e y n k, k <= n ->
+     inc_bound_e_rec k (open_e_rec n (trm_fvar y) e) =
+     open_e_rec (S n) (trm_fvar y) (inc_bound_e_rec k e)).
+Proof.
+  apply typ_trm_mutind; intros; simpl; eauto;
+  try solve [rewrite H; auto; omega];
+  try solve [f_equal; [rewrite H; auto; omega | rewrite H0; auto; omega]].
+  - case_if; case_if; simpl; auto.
+    rewrite If_l in H0; congruence.
+    case_if; simpl; auto. omega.
+Qed.
+
+Lemma inc_bound_open_commute: forall T y n,
+  inc_bound (open_t_rec n (trm_fvar y) T) =
+  open_t_rec (S n) (trm_fvar y) (inc_bound T).
+Proof.
+  intros. unfold inc_bound. apply inc_bound_open_commute_rec.
+  omega.
+Qed.
+
+Lemma open_var_emb_commute: forall T y,
+  (emb_t (T open_tt_var y))=(emb_t T open_t_var y).
+Proof.
+  intros. unfold Fsub.open_tt. unfold Dsub.open_t.
+  remember 0 as n. clear Heqn. generalize dependent n.
+  induction T; intros; eauto.
+  - simpl. case_if; eauto.
+  - simpl. f_equal. rewrite IHT1. reflexivity.
+    rewrite IHT2. rewrite inc_bound_open_commute. reflexivity.
+  - simpl. rewrite IHT1. rewrite IHT2. reflexivity.
+Qed.
+
+Lemma type_inc_bound_noop: forall T,
+  type T ->
+  inc_bound T = T.
+Proof.
+  admit.
+Qed.
+
+Lemma wft_preserved: forall E T,
+  ok (emb_env E) ->
+  Fsub.wft E T ->
+  Dsub.wft (emb_env E) (emb_t T).
+Proof.
+  introv Ok H. induction H; eauto.
+  - simpl. apply wft_sel. right. eexists. reflexivity.
+    eapply wfe_var. eapply binds_sub_preserved; eauto.
+  - simpl. apply wft_all with (L:=dom (emb_env E)); eauto; intros.
+    rewrite open_t_var_type. apply wft_weaken_right.
+    rewrite type_inc_bound_noop. eapply IHwft2; eauto.
+    apply* wft_type. apply ok_push; eauto.
+    rewrite type_inc_bound_noop. apply* wft_type. apply* wft_type.
+  - simpl. apply wft_all with (L:=L \u dom (emb_env E)); eauto. intros y Fry.
+    assert (y \notin L) as Fr by auto. specialize (H1 y Fr).
+    assert (ok (emb_env (E & y ~ bind_sub T1))) as A. {
+      unfold emb_env in *. rewrite map_concat. rewrite map_single.
+      apply ok_push. apply Ok. auto*.
+    }
+    specialize (H1 A). unfold emb_env in *.
+    rewrite map_concat in H1. rewrite map_single in H1. simpl in H1.
+    rewrite open_var_emb_commute in H1. apply H1.
+Qed.
+
+Lemma okt_preserved: forall E,
+  Fsub.okt E ->
+  Dsub.okt (emb_env E).
+Proof.
+  intros. induction E using env_ind.
+  - unfold emb_env. rewrite map_empty. auto.
+  - unfold emb_env. rewrite map_concat. rewrite map_single.
+    destruct (Fsub.okt_push_inv H) as [T [? | ?]]; subst.
+    + destruct (Fsub.okt_push_sub_inv H) as [Ok [Hwf Fr]].
+      apply okt_push; auto.
+      specialize (IHE Ok).
+      assert (ok (emb_env E)) as Ok' by solve [apply* ok_from_okt].
+      lets Hwf': (wft_preserved Ok' Hwf).
+      unfold emb_env in Hwf'. simpl.
+      apply wft_mem. apply Hwf'.
+    + destruct (Fsub.okt_push_typ_inv H) as [Ok [Hwf Fr]].
+      apply okt_push; auto.
+      specialize (IHE Ok).
+      assert (ok (emb_env E)) as Ok' by solve [apply* ok_from_okt].
+      lets Hwf': (wft_preserved Ok' Hwf).
+      unfold emb_env in Hwf'. simpl.
+      apply Hwf'.
+Qed.
+
+Theorem preservation_of_subtyping: forall E S T,
+  Fsub.sub E S T ->
+  Dsub.sub (emb_env E) (emb_t S) (emb_t T).
+Proof.
+  admit.
+Qed.
